Logic/Vorspiel/Meta.lean
@@ -1,0 +1,105 @@
+import Mathlib.Data.Nat.Basic
+import Lean.Elab.Tactic.Basic
+import Mathlib.Tactic.NormNum
+import Mathlib.Tactic.Clear!
+import Mathlib.Util.AtomM
+import Logic.Vorspiel.Vorspiel
+
+open Qq Lean Elab Meta Tactic
+
+universe u v
+
+namespace Qq
+
+def rflQ {α : Q(Sort u)} (a : Q($α)) : Q($a = $a) := q(rfl)
+
+set_option linter.unusedVariables false in
+def decideTQ (p : Q(Prop)) : MetaM Q($p) := do
+  let dec : Q(Decidable $p) ← synthInstanceQ q(Decidable $p)
+  let h : Q(decide $p = true) := rflQ q(true)
+  return q(of_decide_eq_true $h)
+
+def finQVal {n : Q(ℕ)} (e : Q(Fin $n)) : MetaM (Option ℕ) := do
+  let val : Q(ℕ) ← whnf q(Fin.val $e)
+  val.natLit?
+
+-- Returns literal f e when e is literal
+def natAppFunQ (f : ℕ → ℕ) (e : Q(ℕ)) : MetaM Q(ℕ) := do
+  let e : Q(ℕ) ← whnf e
+  let some n := Lean.Expr.natLit? e | throwError "not ℕ"
+  Lean.Expr.ofNat q(ℕ) (f n)
+
+-- https://leanprover-community.github.io/mathlib4_docs//Mathlib/Tactic/Linarith/Verification.html#Qq.inferTypeQ'
+def inferSortQ' (e : Expr) : MetaM ((u : Level) × (α : Q(Sort $u)) × Q($α)) := do
+  let α ← inferType e
+  let .sort u ← instantiateMVars (← whnf (← inferType α))
+    | throwError "not a type{indentExpr α}"
+  pure ⟨u, α, e⟩
+
+-- given an Expr e representing type α : Sort u, returns u and q(α)
+def checkSortQ' (e : Expr) : MetaM (Option ((u : Level) × Q(Sort $u))) := do
+  if let ⟨.succ u, α, e⟩ ← inferSortQ' e then
+    if ← isDefEq α q(Sort $u) then
+      return some ⟨u, e⟩
+    else return none
+  else return none
+
+def inferSortQOfUniverse' (e : Expr) (ty : Q(Sort $u)) : MetaM (Option Q($ty)) := do
+  if let ⟨.succ _, α, e⟩ ← inferSortQ' e then
+    if ← isDefEq α q($ty) then
+      return some e
+    else return none
+  else return none
+
+set_option linter.unusedVariables false in
+def MditeQ {α : Q(Sort u)} (c : Q(Prop)) (dec : Q(Decidable $c)) (t : MetaM Q($c → $α)) (e : MetaM Q(¬$c → $α)) : MetaM Q($α) := do
+  let t ← t
+  let e ← e
+  return q(dite $c (fun h => $t h) (fun h => $e h))
+
+class NormalizeQ (α : Q(Type u)) where
+  normalize : (e : Q($α)) → MetaM ((res : Q($α)) × Q($res = $e))
+
+structure Result (α : Q(Type u)) (e : Q($α)) where
+  expr : Q($α)
+  proof : Q($e = $expr)
+
+namespace Result
+variable  {α : Q(Type u)}
+
+@[reducible] def refl (e : Q($α)) : Result α e := ⟨e, q(rfl)⟩
+
+end Result
+
+set_option linter.unusedVariables false in
+def BEqQ {α : Q(Sort u)} {a b : Q($α)} (h : a == b) : Q($a = $b) := (q(@rfl $α $a) : Expr)
+
+def eqQUnsafe {α : Q(Sort u)} (a b : Q($α)) : Q($a = $b) := (q(@rfl $α $a) : Expr)
+
+def toQList {α : Q(Type u)} : List Q($α) → Q(List $α)
+  | []     => q([])
+  | a :: v => q($a :: $(toQList v))
+
+section List
+variable {α : Type u}
+
+lemma List.mem_of_eq {a b : α} {l} (h : a = b) : a ∈ b :: l := by simp[h]
+
+lemma List.mem_of_mem {a b : α} {l : List α} (h : a ∈ l) : a ∈ b :: l := by simp[h]
+
+def toQListOfElem {α : Q(Type u)} {a : Q($α)} : {l : List Q($α)} → l.elem a → Q($a ∈ $(toQList (u := u) l))
+  | [],     h => by contradiction
+  | b :: l, h =>
+      match be : a == b with
+      | true =>
+        let e : Q($a = $b) := rflQ a
+        q(List.mem_of_eq $e)
+      | false => 
+        let ih : Q($a ∈ $(toQList (u := u) l)) := toQListOfElem (by simpa[be] using h)
+        q(List.mem_of_mem $ih)
+
+example : 2 ∈ [3,4,5,2,6] := of_decide_eq_true rfl
+
+end List
+
+end Qq
